Proofs/e01.lean
@@ -1,10 +1,19 @@
 import examples.e01.translation.Funs
+import Proofs.Anodized
 
 open Aeneas Std.Result
 open e01
 
-theorem f2_anodized_spec (_ : __anodized_fn_requires_f2 = ok true) :
-  f2 ⦃ result =>
-    __anodized_fn_ensures_f2 result = ok true⦄ := by
-  unfold f2 __anodized_fn_ensures_f2 __anodized_fn_ensures_f2.closure.Insts.CoreOpsFunctionFnTupleSharedU8Bool.call
+register_anodized_simps
+
+theorem f2_spec : Anodized f2 := by
+  intro _
+  unfold f2
+  step*
+
+theorem f4_spec : Anodized f4 := by
+  intro x hx
+  -- precondition `x > 0`
+  simp only [step_simps] at hx
+  unfold f4
   step*
